raw rsa restruct

dist/gcc-compatible/lib/Hacl_RSAPSS_bindings.ml
@@ -27,19 +27,6 @@ module Bindings(F:Cstubs.FOREIGN) =
                        (uint32_t @->
                           (ocaml_bytes @->
                              (uint32_t @-> (ocaml_bytes @-> (returning bool))))))))))
-    let hacl_RSAPSS_new_rsapss_load_pkey =
-      foreign "Hacl_RSAPSS_new_rsapss_load_pkey"
-        (uint32_t @->
-           (uint32_t @->
-              (ocaml_bytes @-> (ocaml_bytes @-> (returning (ptr uint64_t))))))
-    let hacl_RSAPSS_new_rsapss_load_skey =
-      foreign "Hacl_RSAPSS_new_rsapss_load_skey"
-        (uint32_t @->
-           (uint32_t @->
-              (uint32_t @->
-                 (ocaml_bytes @->
-                    (ocaml_bytes @->
-                       (ocaml_bytes @-> (returning (ptr uint64_t))))))))
     let hacl_RSAPSS_rsapss_skey_sign =
       foreign "Hacl_RSAPSS_rsapss_skey_sign"
         (spec_Hash_Definitions_hash_alg @->
