dist/msvc-compatible/Hacl_RSAPSS.c
@@ -25,6 +25,7 @@
 
 #include "Hacl_RSAPSS.h"
 
+#include "internal/Hacl_RSA.h"
 #include "internal/Hacl_Krmllib.h"
 #include "internal/Hacl_Bignum_Base.h"
 #include "internal/Hacl_Bignum.h"
@@ -147,73 +148,6 @@ mgf_hash(
     hash(a, acc_i, len + 4U, mgfseed_counter);
   }
   memcpy(res, acc, maskLen * sizeof (uint8_t));
-}
-
-static inline uint64_t check_num_bits_u64(uint32_t bs, uint64_t *b)
-{
-  uint32_t bLen = (bs - 1U) / 64U + 1U;
-  if (bs == 64U * bLen)
-  {
-    return 0xFFFFFFFFFFFFFFFFULL;
-  }
-  KRML_CHECK_SIZE(sizeof (uint64_t), bLen);
-  uint64_t *b2 = (uint64_t *)alloca(bLen * sizeof (uint64_t));
-  memset(b2, 0U, bLen * sizeof (uint64_t));
-  uint32_t i0 = bs / 64U;
-  uint32_t j = bs % 64U;
-  b2[i0] = b2[i0] | 1ULL << j;
-  uint64_t acc = 0ULL;
-  for (uint32_t i = 0U; i < bLen; i++)
-  {
-    uint64_t beq = FStar_UInt64_eq_mask(b[i], b2[i]);
-    uint64_t blt = ~FStar_UInt64_gte_mask(b[i], b2[i]);
-    acc = (beq & acc) | (~beq & ((blt & 0xFFFFFFFFFFFFFFFFULL) | (~blt & 0ULL)));
-  }
-  uint64_t res = acc;
-  return res;
-}
-
-static inline uint64_t check_modulus_u64(uint32_t modBits, uint64_t *n)
-{
-  uint32_t nLen = (modBits - 1U) / 64U + 1U;
-  uint64_t bits0 = n[0U] & 1ULL;
-  uint64_t m0 = 0ULL - bits0;
-  KRML_CHECK_SIZE(sizeof (uint64_t), nLen);
-  uint64_t *b2 = (uint64_t *)alloca(nLen * sizeof (uint64_t));
-  memset(b2, 0U, nLen * sizeof (uint64_t));
-  uint32_t i0 = (modBits - 1U) / 64U;
-  uint32_t j = (modBits - 1U) % 64U;
-  b2[i0] = b2[i0] | 1ULL << j;
-  uint64_t acc = 0ULL;
-  for (uint32_t i = 0U; i < nLen; i++)
-  {
-    uint64_t beq = FStar_UInt64_eq_mask(b2[i], n[i]);
-    uint64_t blt = ~FStar_UInt64_gte_mask(b2[i], n[i]);
-    acc = (beq & acc) | (~beq & ((blt & 0xFFFFFFFFFFFFFFFFULL) | (~blt & 0ULL)));
-  }
-  uint64_t res = acc;
-  uint64_t m1 = res;
-  uint64_t m2 = check_num_bits_u64(modBits, n);
-  return m0 & (m1 & m2);
-}
-
-static inline uint64_t check_exponent_u64(uint32_t eBits, uint64_t *e)
-{
-  uint32_t eLen = (eBits - 1U) / 64U + 1U;
-  KRML_CHECK_SIZE(sizeof (uint64_t), eLen);
-  uint64_t *bn_zero = (uint64_t *)alloca(eLen * sizeof (uint64_t));
-  memset(bn_zero, 0U, eLen * sizeof (uint64_t));
-  uint64_t mask = 0xFFFFFFFFFFFFFFFFULL;
-  for (uint32_t i = 0U; i < eLen; i++)
-  {
-    uint64_t uu____0 = FStar_UInt64_eq_mask(e[i], bn_zero[i]);
-    mask = uu____0 & mask;
-  }
-  uint64_t mask1 = mask;
-  uint64_t res = mask1;
-  uint64_t m0 = res;
-  uint64_t m1 = check_num_bits_u64(eBits, e);
-  return ~m0 & m1;
 }
 
 static inline void
@@ -366,8 +300,8 @@ load_pkey(uint32_t modBits, uint32_t eBits, uint8_t *nb, uint8_t *eb, uint64_t *
   Hacl_Bignum_Convert_bn_from_bytes_be_uint64(nbLen, nb, n);
   Hacl_Bignum_Montgomery_bn_precomp_r2_mod_n_u64((modBits - 1U) / 64U + 1U, modBits - 1U, n, r2);
   Hacl_Bignum_Convert_bn_from_bytes_be_uint64(ebLen, eb, e);
-  uint64_t m0 = check_modulus_u64(modBits, n);
-  uint64_t m1 = check_exponent_u64(eBits, e);
+  uint64_t m0 = Hacl_Impl_RSA_Keys_check_modulus_u64(modBits, n);
+  uint64_t m1 = Hacl_Impl_RSA_Keys_check_exponent_u64(eBits, e);
   uint64_t m = m0 & m1;
   return m == 0xFFFFFFFFFFFFFFFFULL;
 }
@@ -391,7 +325,7 @@ load_skey(
   uint64_t *d = skey + pkeyLen;
   bool b = load_pkey(modBits, eBits, nb, eb, pkey);
   Hacl_Bignum_Convert_bn_from_bytes_be_uint64(dbLen, db, d);
-  uint64_t m1 = check_exponent_u64(dBits, d);
+  uint64_t m1 = Hacl_Impl_RSA_Keys_check_exponent_u64(dBits, d);
   return b && m1 == 0xFFFFFFFFFFFFFFFFULL;
 }
 
@@ -433,68 +367,14 @@ Hacl_RSAPSS_rsapss_sign(
   b = saltLen <= 0xffffffffU - hLen - 8U && saltLen + hLen + 2U <= (modBits - 1U - 1U) / 8U + 1U;
   if (b)
   {
-    uint32_t nLen = (modBits - 1U) / 64U + 1U;
-    KRML_CHECK_SIZE(sizeof (uint64_t), nLen);
-    uint64_t *m = (uint64_t *)alloca(nLen * sizeof (uint64_t));
-    memset(m, 0U, nLen * sizeof (uint64_t));
-    uint32_t emBits = modBits - 1U;
-    uint32_t emLen = (emBits - 1U) / 8U + 1U;
+    uint32_t emLen = (modBits - 1U - 1U) / 8U + 1U;
     KRML_CHECK_SIZE(sizeof (uint8_t), emLen);
     uint8_t *em = (uint8_t *)alloca(emLen * sizeof (uint8_t));
     memset(em, 0U, emLen * sizeof (uint8_t));
+    uint32_t emBits = modBits - 1U;
     pss_encode(a, saltLen, salt, msgLen, msg, emBits, em);
-    Hacl_Bignum_Convert_bn_from_bytes_be_uint64(emLen, em, m);
-    uint32_t nLen1 = (modBits - 1U) / 64U + 1U;
-    uint32_t k = (modBits - 1U) / 8U + 1U;
-    KRML_CHECK_SIZE(sizeof (uint64_t), nLen1);
-    uint64_t *s = (uint64_t *)alloca(nLen1 * sizeof (uint64_t));
-    memset(s, 0U, nLen1 * sizeof (uint64_t));
-    KRML_CHECK_SIZE(sizeof (uint64_t), nLen1);
-    uint64_t *m_ = (uint64_t *)alloca(nLen1 * sizeof (uint64_t));
-    memset(m_, 0U, nLen1 * sizeof (uint64_t));
-    uint32_t nLen2 = (modBits - 1U) / 64U + 1U;
-    uint32_t eLen = (eBits - 1U) / 64U + 1U;
-    uint64_t *n = skey;
-    uint64_t *r2 = skey + nLen2;
-    uint64_t *e = skey + nLen2 + nLen2;
-    uint64_t *d = skey + nLen2 + nLen2 + eLen;
-    uint64_t mu = Hacl_Bignum_ModInvLimb_mod_inv_uint64(n[0U]);
-    Hacl_Bignum_Exponentiation_bn_mod_exp_consttime_precomp_u64((modBits - 1U) / 64U + 1U,
-      n,
-      mu,
-      r2,
-      m,
-      dBits,
-      d,
-      s);
-    uint64_t mu0 = Hacl_Bignum_ModInvLimb_mod_inv_uint64(n[0U]);
-    Hacl_Bignum_Exponentiation_bn_mod_exp_vartime_precomp_u64((modBits - 1U) / 64U + 1U,
-      n,
-      mu0,
-      r2,
-      s,
-      eBits,
-      e,
-      m_);
-    uint64_t mask = 0xFFFFFFFFFFFFFFFFULL;
-    for (uint32_t i = 0U; i < nLen2; i++)
-    {
-      uint64_t uu____0 = FStar_UInt64_eq_mask(m[i], m_[i]);
-      mask = uu____0 & mask;
-    }
-    uint64_t mask1 = mask;
-    uint64_t eq_m = mask1;
-    for (uint32_t i = 0U; i < nLen2; i++)
-    {
-      uint64_t *os = s;
-      uint64_t x = s[i];
-      uint64_t x0 = eq_m & x;
-      os[i] = x0;
-    }
-    bool eq_b = eq_m == 0xFFFFFFFFFFFFFFFFULL;
-    Hacl_Bignum_Convert_bn_to_bytes_be_uint64(k, s, sgnt);
-    bool eq_b0 = eq_b;
-    return eq_b0;
+    bool eq_b = Hacl_RSA_rsa_dec(modBits, eBits, dBits, skey, em, sgnt);
+    return eq_b;
   }
   return false;
 }
@@ -534,234 +414,21 @@ Hacl_RSAPSS_rsapss_verify(
   bool b = saltLen <= 0xffffffffU - hLen - 8U && sgntLen == (modBits - 1U) / 8U + 1U;
   if (b)
   {
-    uint32_t nLen = (modBits - 1U) / 64U + 1U;
-    KRML_CHECK_SIZE(sizeof (uint64_t), nLen);
-    uint64_t *m = (uint64_t *)alloca(nLen * sizeof (uint64_t));
-    memset(m, 0U, nLen * sizeof (uint64_t));
-    uint32_t nLen1 = (modBits - 1U) / 64U + 1U;
-    uint32_t k = (modBits - 1U) / 8U + 1U;
-    KRML_CHECK_SIZE(sizeof (uint64_t), nLen1);
-    uint64_t *s = (uint64_t *)alloca(nLen1 * sizeof (uint64_t));
-    memset(s, 0U, nLen1 * sizeof (uint64_t));
-    Hacl_Bignum_Convert_bn_from_bytes_be_uint64(k, sgnt, s);
-    uint32_t nLen2 = (modBits - 1U) / 64U + 1U;
-    uint64_t *n = pkey;
-    uint64_t *r2 = pkey + nLen2;
-    uint64_t *e = pkey + nLen2 + nLen2;
-    uint64_t acc = 0ULL;
-    for (uint32_t i = 0U; i < nLen2; i++)
+    uint32_t emBits = modBits - 1U;
+    uint32_t emLen = (emBits - 1U) / 8U + 1U;
+    KRML_CHECK_SIZE(sizeof (uint8_t), emLen);
+    uint8_t *em = (uint8_t *)alloca(emLen * sizeof (uint8_t));
+    memset(em, 0U, emLen * sizeof (uint8_t));
+    bool b1 = Hacl_RSA_rsa_enc(modBits, eBits, pkey, sgnt, em);
+    if (b1)
     {
-      uint64_t beq = FStar_UInt64_eq_mask(s[i], n[i]);
-      uint64_t blt = ~FStar_UInt64_gte_mask(s[i], n[i]);
-      acc = (beq & acc) | (~beq & ((blt & 0xFFFFFFFFFFFFFFFFULL) | (~blt & 0ULL)));
-    }
-    uint64_t mask = acc;
-    bool res;
-    if (mask == 0xFFFFFFFFFFFFFFFFULL)
-    {
-      uint64_t mu = Hacl_Bignum_ModInvLimb_mod_inv_uint64(n[0U]);
-      Hacl_Bignum_Exponentiation_bn_mod_exp_vartime_precomp_u64((modBits - 1U) / 64U + 1U,
-        n,
-        mu,
-        r2,
-        s,
-        eBits,
-        e,
-        m);
-      bool ite;
-      if (!((modBits - 1U) % 8U == 0U))
-      {
-        ite = true;
-      }
-      else
-      {
-        uint32_t i = (modBits - 1U) / 64U;
-        uint32_t j = (modBits - 1U) % 64U;
-        uint64_t tmp = m[i];
-        uint64_t get_bit = tmp >> j & 1ULL;
-        ite = get_bit == 0ULL;
-      }
-      if (ite)
-      {
-        res = true;
-      }
-      else
-      {
-        res = false;
-      }
-    }
-    else
-    {
-      res = false;
-    }
-    bool b1 = res;
-    bool b10 = b1;
-    if (b10)
-    {
-      uint32_t emBits = modBits - 1U;
-      uint32_t emLen = (emBits - 1U) / 8U + 1U;
-      KRML_CHECK_SIZE(sizeof (uint8_t), emLen);
-      uint8_t *em = (uint8_t *)alloca(emLen * sizeof (uint8_t));
-      memset(em, 0U, emLen * sizeof (uint8_t));
-      uint64_t *m1 = m;
-      Hacl_Bignum_Convert_bn_to_bytes_be_uint64(emLen, m1, em);
-      bool res0 = pss_verify(a, saltLen, msgLen, msg, emBits, em);
-      return res0;
+      uint32_t emBits1 = modBits - 1U;
+      bool res = pss_verify(a, saltLen, msgLen, msg, emBits1, em);
+      return res;
     }
     return false;
   }
   return false;
-}
-
-/**
-Load a public key from key parts.
-
-@param modBits Count of bits in modulus (`n`).
-@param eBits Count of bits in `e` value.
-@param nb Pointer to `ceil(modBits / 8)` bytes where the modulus (`n`), in big-endian byte order, is read from.
-@param eb Pointer to `ceil(modBits / 8)` bytes where the `e` value, in big-endian byte order, is read from.
-
-@return Returns an allocated public key upon success, otherwise, `NULL` if key part arguments are invalid or memory allocation fails. Note: caller must take care to `free()` the created key.
-*/
-uint64_t
-*Hacl_RSAPSS_new_rsapss_load_pkey(uint32_t modBits, uint32_t eBits, uint8_t *nb, uint8_t *eb)
-{
-  bool ite;
-  if (1U < modBits && 0U < eBits)
-  {
-    uint32_t nLen = (modBits - 1U) / 64U + 1U;
-    uint32_t eLen = (eBits - 1U) / 64U + 1U;
-    ite = nLen <= 33554431U && eLen <= 67108863U && nLen + nLen <= 0xffffffffU - eLen;
-  }
-  else
-  {
-    ite = false;
-  }
-  if (!ite)
-  {
-    return NULL;
-  }
-  uint32_t nLen = (modBits - 1U) / 64U + 1U;
-  uint32_t eLen = (eBits - 1U) / 64U + 1U;
-  uint32_t pkeyLen = nLen + nLen + eLen;
-  KRML_CHECK_SIZE(sizeof (uint64_t), pkeyLen);
-  uint64_t *pkey = (uint64_t *)KRML_HOST_CALLOC(pkeyLen, sizeof (uint64_t));
-  if (pkey == NULL)
-  {
-    return pkey;
-  }
-  uint64_t *pkey1 = pkey;
-  uint64_t *pkey2 = pkey1;
-  uint32_t nbLen = (modBits - 1U) / 8U + 1U;
-  uint32_t ebLen = (eBits - 1U) / 8U + 1U;
-  uint32_t nLen1 = (modBits - 1U) / 64U + 1U;
-  uint64_t *n = pkey2;
-  uint64_t *r2 = pkey2 + nLen1;
-  uint64_t *e = pkey2 + nLen1 + nLen1;
-  Hacl_Bignum_Convert_bn_from_bytes_be_uint64(nbLen, nb, n);
-  Hacl_Bignum_Montgomery_bn_precomp_r2_mod_n_u64((modBits - 1U) / 64U + 1U, modBits - 1U, n, r2);
-  Hacl_Bignum_Convert_bn_from_bytes_be_uint64(ebLen, eb, e);
-  uint64_t m0 = check_modulus_u64(modBits, n);
-  uint64_t m1 = check_exponent_u64(eBits, e);
-  uint64_t m = m0 & m1;
-  bool b = m == 0xFFFFFFFFFFFFFFFFULL;
-  if (b)
-  {
-    return pkey2;
-  }
-  KRML_HOST_FREE(pkey2);
-  return NULL;
-}
-
-/**
-Load a secret key from key parts.
-
-@param modBits Count of bits in modulus (`n`).
-@param eBits Count of bits in `e` value.
-@param dBits Count of bits in `d` value.
-@param nb Pointer to `ceil(modBits / 8)` bytes where the modulus (`n`), in big-endian byte order, is read from.
-@param eb Pointer to `ceil(modBits / 8)` bytes where the `e` value, in big-endian byte order, is read from.
-@param db Pointer to `ceil(modBits / 8)` bytes where the `d` value, in big-endian byte order, is read from.
-
-@return Returns an allocated secret key upon success, otherwise, `NULL` if key part arguments are invalid or memory allocation fails. Note: caller must take care to `free()` the created key.
-*/
-uint64_t
-*Hacl_RSAPSS_new_rsapss_load_skey(
-  uint32_t modBits,
-  uint32_t eBits,
-  uint32_t dBits,
-  uint8_t *nb,
-  uint8_t *eb,
-  uint8_t *db
-)
-{
-  bool ite0;
-  if (1U < modBits && 0U < eBits)
-  {
-    uint32_t nLen = (modBits - 1U) / 64U + 1U;
-    uint32_t eLen = (eBits - 1U) / 64U + 1U;
-    ite0 = nLen <= 33554431U && eLen <= 67108863U && nLen + nLen <= 0xffffffffU - eLen;
-  }
-  else
-  {
-    ite0 = false;
-  }
-  bool ite;
-  if (ite0 && 0U < dBits)
-  {
-    uint32_t nLen = (modBits - 1U) / 64U + 1U;
-    uint32_t eLen = (eBits - 1U) / 64U + 1U;
-    uint32_t dLen = (dBits - 1U) / 64U + 1U;
-    ite = dLen <= 67108863U && 2U * nLen <= 0xffffffffU - eLen - dLen;
-  }
-  else
-  {
-    ite = false;
-  }
-  if (!ite)
-  {
-    return NULL;
-  }
-  uint32_t nLen = (modBits - 1U) / 64U + 1U;
-  uint32_t eLen = (eBits - 1U) / 64U + 1U;
-  uint32_t dLen = (dBits - 1U) / 64U + 1U;
-  uint32_t skeyLen = nLen + nLen + eLen + dLen;
-  KRML_CHECK_SIZE(sizeof (uint64_t), skeyLen);
-  uint64_t *skey = (uint64_t *)KRML_HOST_CALLOC(skeyLen, sizeof (uint64_t));
-  if (skey == NULL)
-  {
-    return skey;
-  }
-  uint64_t *skey1 = skey;
-  uint64_t *skey2 = skey1;
-  uint32_t dbLen = (dBits - 1U) / 8U + 1U;
-  uint32_t nLen1 = (modBits - 1U) / 64U + 1U;
-  uint32_t eLen1 = (eBits - 1U) / 64U + 1U;
-  uint32_t pkeyLen = nLen1 + nLen1 + eLen1;
-  uint64_t *pkey = skey2;
-  uint64_t *d = skey2 + pkeyLen;
-  uint32_t nbLen1 = (modBits - 1U) / 8U + 1U;
-  uint32_t ebLen1 = (eBits - 1U) / 8U + 1U;
-  uint32_t nLen2 = (modBits - 1U) / 64U + 1U;
-  uint64_t *n = pkey;
-  uint64_t *r2 = pkey + nLen2;
-  uint64_t *e = pkey + nLen2 + nLen2;
-  Hacl_Bignum_Convert_bn_from_bytes_be_uint64(nbLen1, nb, n);
-  Hacl_Bignum_Montgomery_bn_precomp_r2_mod_n_u64((modBits - 1U) / 64U + 1U, modBits - 1U, n, r2);
-  Hacl_Bignum_Convert_bn_from_bytes_be_uint64(ebLen1, eb, e);
-  uint64_t m0 = check_modulus_u64(modBits, n);
-  uint64_t m10 = check_exponent_u64(eBits, e);
-  uint64_t m = m0 & m10;
-  bool b = m == 0xFFFFFFFFFFFFFFFFULL;
-  Hacl_Bignum_Convert_bn_from_bytes_be_uint64(dbLen, db, d);
-  uint64_t m1 = check_exponent_u64(dBits, d);
-  bool b0 = b && m1 == 0xFFFFFFFFFFFFFFFFULL;
-  if (b0)
-  {
-    return skey2;
-  }
-  KRML_HOST_FREE(skey2);
-  return NULL;
 }
 
 /**
