code/rsapss/Hacl.Impl.RSAPSS.fst
@@ -28,157 +28,42 @@ module LSeq = Lib.Sequence
 
 module RP = Hacl.Impl.RSAPSS.Padding
 module RM = Hacl.Impl.RSAPSS.MGF
-module RK = Hacl.Impl.RSAPSS.Keys
+module RK = Hacl.Impl.RSA.Keys
+open Hacl.Impl.RSA
 
 #reset-options "--z3rlimit 150 --fuel 0 --ifuel 0"
 
-inline_for_extraction noextract
-let modBits_t (t:limb_t) = modBits:size_t{1 < v modBits /\ 2 * bits t * SD.blocks (v modBits) (bits t) <= max_size_t}
-
 
 inline_for_extraction noextract
-let rsapss_sign_bn_st (t:limb_t) (ke:BE.exp t) (modBits:modBits_t t) =
-  let len = blocks modBits (size (bits t)) in
-    eBits:size_t
-  -> dBits:size_t{LS.skey_len_pre t (v modBits) (v eBits) (v dBits)}
-  -> skey:lbignum t (2ul *! len +! blocks eBits (size (bits t)) +! blocks dBits (size (bits t)))
-  -> m:lbignum t len
-  -> m':lbignum t len
-  -> s:lbignum t len ->
-  Stack bool
-  (requires fun h -> len == ke.BE.bn.BN.len /\
-    live h skey /\ live h m /\ live h s /\ live h m' /\
-    disjoint s m /\ disjoint s skey /\ disjoint m skey /\
-    disjoint m m' /\ disjoint m' s /\ disjoint m' skey /\
-    LS.rsapss_skey_pre (v modBits) (v eBits) (v dBits) (as_seq h skey) /\
-    bn_v h m < bn_v h (gsub skey 0ul len))
-  (ensures  fun h0 r h1 -> modifies (loc s |+| loc m') h0 h1 /\
-    (r, as_seq h1 s) == LS.rsapss_sign_bn (v modBits) (v eBits) (v dBits) (as_seq h0 skey) (as_seq h0 m))
-
-
-inline_for_extraction noextract
-val rsapss_sign_bn: #t:limb_t -> ke:BE.exp t -> modBits:modBits_t t -> rsapss_sign_bn_st t ke modBits
-let rsapss_sign_bn #t ke modBits eBits dBits skey m m' s =
-  [@inline_let] let bits : size_pos = bits t in
-  let nLen = blocks modBits (size bits) in
-  let eLen = blocks eBits (size bits) in
-  let dLen = blocks dBits (size bits) in
-
-  let n  = sub skey 0ul nLen in
-  let r2 = sub skey nLen nLen in
-  let e  = sub skey (nLen +! nLen) eLen in
-  let d  = sub skey (nLen +! nLen +! eLen) dLen in
-
-  Math.Lemmas.pow2_le_compat (bits * v nLen) (v modBits);
-  let h0 = ST.get () in
-  SM.bn_precomp_r2_mod_n_lemma (v modBits - 1) (as_seq h0 n);
-  BE.mk_bn_mod_exp_precompr2 nLen ke.BE.exp_ct_precomp n r2 m dBits d s;
-  BE.mk_bn_mod_exp_precompr2 nLen ke.BE.exp_vt_precomp n r2 s eBits e m';
-  let h1 = ST.get () in
-  SD.bn_eval_inj (v nLen) (as_seq h1 s)
-    (SE.bn_mod_exp_consttime_precompr2 (v nLen) (as_seq h0 n) (as_seq h0 r2)
-    (as_seq h0 m) (v dBits) (as_seq h0 d));
-  SD.bn_eval_inj (v nLen) (as_seq h1 m')
-    (SE.bn_mod_exp_vartime_precompr2 (v nLen) (as_seq h0 n) (as_seq h0 r2)
-    (as_seq h1 s) (v eBits) (as_seq h0 e));
-  let eq_m = BN.bn_eq_mask nLen m m' in
-  mapT nLen s (logand eq_m) s;
-  BB.unsafe_bool_of_limb eq_m
-
-
-inline_for_extraction noextract
-let rsapss_sign_msg_to_bn_st (t:limb_t) (a:Hash.hash_alg{S.hash_is_supported a}) (modBits:modBits_t t) =
-  let len = blocks modBits (size (bits t)) in
+let rsapss_encode_msg_st (t:limb_t) (a:Hash.hash_alg{S.hash_is_supported a}) (modBits:modBits_t t) =
+  let len = blocks (modBits -! 1ul) 8ul in
     saltLen:size_t
   -> salt:lbuffer uint8 saltLen
   -> msgLen:size_t
   -> msg:lbuffer uint8 msgLen
-  -> m:lbignum t len ->
+  -> em:lbuffer uint8 len ->
   Stack unit
   (requires fun h ->
-    live h salt /\ live h msg /\ live h m /\
-    disjoint salt msg /\ disjoint m msg /\ disjoint m salt /\
-    as_seq h m == LSeq.create (v len) (uint #t 0) /\
+    live h salt /\ live h msg /\ live h em /\
+    disjoint salt msg /\ disjoint em msg /\ disjoint em salt /\
+    as_seq h em == LSeq.create (v len) (u8 0) /\
     LS.rsapss_sign_pre a (v modBits) (v saltLen) (as_seq h salt) (v msgLen) (as_seq h msg))
-  (ensures  fun h0 _ h1 -> modifies (loc m) h0 h1 /\
-    as_seq h1 m == LS.rsapss_sign_msg_to_bn a (v modBits) (v saltLen) (as_seq h0 salt) (v msgLen) (as_seq h0 msg))
+  (ensures  fun h0 _ h1 -> modifies (loc em) h0 h1 /\
+    as_seq h1 em == LS.rsapss_encode_msg a (v modBits) (v saltLen) (as_seq h0 salt) (v msgLen) (as_seq h0 msg))
 
 
 inline_for_extraction noextract
-val rsapss_sign_msg_to_bn:
+val rsapss_encode_msg:
     #t:limb_t
   -> a:Hash.hash_alg{S.hash_is_supported a}
   -> modBits:modBits_t t ->
-  rsapss_sign_msg_to_bn_st t a modBits
+    rsapss_encode_msg_st t a modBits
 
-let rsapss_sign_msg_to_bn #t a modBits saltLen salt msgLen msg m =
-  push_frame ();
-  [@inline_let] let bits : size_pos = bits t in
-  [@inline_let] let numb : size_pos = numbytes t in
-  let nLen = blocks modBits (size bits) in
-
+let rsapss_encode_msg #t a modBits saltLen salt msgLen msg em =
   let emBits = modBits -! 1ul in
   let emLen = blocks emBits 8ul in
-  [@inline_let] let mLen = blocks emLen (size numb) in
+  RP.pss_encode a saltLen salt msgLen msg emBits em
 
-  let em = create emLen (u8 0) in
-  RP.pss_encode a saltLen salt msgLen msg emBits em;
-  LS.blocks_bits_lemma t (v emBits);
-  LS.blocks_numb_lemma t (v emBits);
-  assert (SD.blocks (v emBits) bits = v mLen);
-  assert (numb * v mLen <= max_size_t);
-  assert (v mLen <= v nLen);
-
-  let h' = ST.get () in
-  update_sub_f h' m 0ul mLen
-    (fun h -> SB.bn_from_bytes_be (v emLen) (as_seq h' em))
-    (fun _ -> BN.bn_from_bytes_be emLen em (sub m 0ul mLen));
-  pop_frame ()
-
-
-inline_for_extraction noextract
-let rsapss_sign_compute_sgnt_st (t:limb_t) (ke:BE.exp t) (modBits:modBits_t t) =
-  let len = blocks modBits (size (bits t)) in
-    eBits:size_t
-  -> dBits:size_t{LS.skey_len_pre t (v modBits) (v eBits) (v dBits)}
-  -> skey:lbignum t (2ul *! len +! blocks eBits (size (bits t)) +! blocks dBits (size (bits t)))
-  -> m:lbignum t len
-  -> sgnt:lbuffer uint8 (blocks modBits 8ul) ->
-  Stack bool
-  (requires fun h -> len == ke.BE.bn.BN.len /\
-    live h sgnt /\ live h skey /\ live h m /\
-    disjoint sgnt skey /\ disjoint m sgnt /\ disjoint m skey /\
-    LS.rsapss_skey_pre (v modBits) (v eBits) (v dBits) (as_seq h skey) /\
-    bn_v h m < bn_v h (gsub skey 0ul len))
-  (ensures  fun h0 eq_m h1 -> modifies (loc sgnt) h0 h1 /\
-    (eq_m, as_seq h1 sgnt) == LS.rsapss_sign_compute_sgnt (v modBits) (v eBits) (v dBits) (as_seq h0 skey) (as_seq h0 m))
-
-
-inline_for_extraction noextract
-val rsapss_sign_compute_sgnt:
-    #t:limb_t
-  -> ke:BE.exp t
-  -> modBits:modBits_t t ->
-  rsapss_sign_compute_sgnt_st t ke modBits
-
-let rsapss_sign_compute_sgnt #t ke modBits eBits dBits skey m sgnt =
-  push_frame ();
-  let h_init = ST.get () in
-  [@inline_let] let bits : size_pos = bits t in
-  [@inline_let] let numb : size_pos = numbytes t in
-  let nLen = blocks modBits (size bits) in
-
-  let k = blocks modBits 8ul in
-  let s = create nLen (uint #t 0) in
-  let m' = create nLen (uint #t 0) in
-  let eq_b = rsapss_sign_bn ke modBits eBits dBits skey m m' s in
-  LS.blocks_bits_lemma t (v modBits);
-  LS.blocks_numb_lemma t (v modBits);
-  assert (SD.blocks (v k) numb == v nLen);
-  assert (numb * v nLen <= max_size_t);
-  BN.bn_to_bytes_be k s sgnt;
-  pop_frame ();
-  eq_b
 
 
 inline_for_extraction noextract
@@ -198,7 +83,7 @@ let rsapss_sign_st1 (t:limb_t) (ke:BE.exp t) (a:Hash.hash_alg{S.hash_is_supporte
     disjoint sgnt salt /\ disjoint sgnt msg /\ disjoint sgnt salt /\ disjoint sgnt skey /\
     disjoint salt msg /\
 
-    LS.rsapss_skey_pre (v modBits) (v eBits) (v dBits) (as_seq h skey) /\
+    LS.rsa_skey_pre (v modBits) (v eBits) (v dBits) (as_seq h skey) /\
     LS.rsapss_sign_pre a (v modBits) (v saltLen) (as_seq h salt) (v msgLen) (as_seq h msg))
   (ensures  fun h0 eq_m h1 -> modifies (loc sgnt) h0 h1 /\
     (eq_m, as_seq h1 sgnt) == LS.rsapss_sign_ a (v modBits) (v eBits) (v dBits)
@@ -210,16 +95,16 @@ val rsapss_sign_:
     #t:limb_t
   -> ke:BE.exp t
   -> a:Hash.hash_alg{S.hash_is_supported a}
-  -> modBits:modBits_t t ->
+  -> modBits:modBits_t t
+  -> rsa_dec:rsa_dec_st t ke modBits ->
   rsapss_sign_st1 t ke a modBits
 
-let rsapss_sign_ #t ke a modBits eBits dBits skey saltLen salt msgLen msg sgnt =
-  push_frame ();
-  [@inline_let] let bits : size_pos = bits t in
-  let nLen = blocks modBits (size bits) in
-  let m = create nLen (uint #t 0) in
-  rsapss_sign_msg_to_bn a modBits saltLen salt msgLen msg m;
-  let eq_b = rsapss_sign_compute_sgnt ke modBits eBits dBits skey m sgnt in
+let rsapss_sign_ #t ke a modBits rsa_dec eBits dBits skey saltLen salt msgLen msg sgnt =
+  push_frame (); 
+  let emLen = blocks (modBits -! 1ul) 8ul in
+  let em = create emLen (u8 0) in
+  rsapss_encode_msg a modBits saltLen salt msgLen msg em;
+  let eq_b = rsa_dec eBits dBits skey em sgnt in
   pop_frame ();
   eq_b
 
@@ -241,7 +126,7 @@ let rsapss_sign_st (t:limb_t) (ke:BE.exp t) (a:Hash.hash_alg{S.hash_is_supported
     disjoint sgnt salt /\ disjoint sgnt msg /\ disjoint sgnt salt /\ disjoint sgnt skey /\
     disjoint salt msg /\
 
-    LS.rsapss_skey_pre (v modBits) (v eBits) (v dBits) (as_seq h skey))
+    LS.rsa_skey_pre (v modBits) (v eBits) (v dBits) (as_seq h skey))
   (ensures  fun h0 b h1 -> modifies (loc sgnt) h0 h1 /\
     (b, as_seq h1 sgnt) == LS.rsapss_sign a (v modBits) (v eBits) (v dBits)
       (as_seq h0 skey) (v saltLen) (as_seq h0 salt) (v msgLen) (as_seq h0 msg) (as_seq h0 sgnt))
@@ -252,10 +137,11 @@ val rsapss_sign:
     #t:limb_t
   -> ke:BE.exp t
   -> a:Hash.hash_alg{S.hash_is_supported a}
-  -> modBits:modBits_t t ->
+  -> modBits:modBits_t t
+  -> rsa_dec:rsa_dec_st t ke modBits ->
   rsapss_sign_st t ke a modBits
 
-let rsapss_sign #t ke a modBits eBits dBits skey saltLen salt msgLen msg sgnt =
+let rsapss_sign #t ke a modBits rsa_dec eBits dBits skey saltLen salt msgLen msg sgnt =
   let hLen = RM.hash_len a in
   Math.Lemmas.pow2_lt_compat 61 32;
   Math.Lemmas.pow2_lt_compat 125 32;
@@ -266,165 +152,37 @@ let rsapss_sign #t ke a modBits eBits dBits skey saltLen salt msgLen msg sgnt =
     saltLen +! hLen +! 2ul <=. blocks (modBits -! 1ul) 8ul in
 
   if b then
-    rsapss_sign_ ke a modBits eBits dBits skey saltLen salt msgLen msg sgnt
+    rsapss_sign_ ke a modBits rsa_dec eBits dBits skey saltLen salt msgLen msg sgnt
   else
     false
 
-
-
 inline_for_extraction noextract
-val bn_lt_pow2:
-    #t:limb_t
-  -> modBits:size_t{1 < v modBits}
-  -> m:lbignum t (blocks modBits (size (bits t))) ->
-  Stack bool
-  (requires fun h -> live h m)
-  (ensures  fun h0 r h1 -> h0 == h1 /\
-    r == LS.bn_lt_pow2 (v modBits) (as_seq h0 m))
-
-let bn_lt_pow2 #t modBits m =
-  if not ((modBits -! 1ul) %. 8ul =. 0ul) then true
-  else begin
-    let get_bit = BN.bn_get_ith_bit (blocks modBits (size (bits t))) m (modBits -! 1ul) in
-    BB.unsafe_bool_of_limb0 get_bit end
-
-
-inline_for_extraction noextract
-let rsapss_verify_bn_st (t:limb_t) (ke:BE.exp t) (modBits:modBits_t t) =
-  let len = blocks modBits (size (bits t)) in
-    eBits:size_t{LS.pkey_len_pre t (v modBits) (v eBits)}
-  -> pkey:lbignum t (2ul *! len +! blocks eBits (size (bits t)))
-  -> m_def:lbignum t len
-  -> s:lbignum t len ->
-  Stack bool
-  (requires fun h -> len == ke.BE.bn.BN.len /\
-    live h pkey /\ live h m_def /\ live h s /\
-    disjoint m_def pkey /\ disjoint m_def s /\ disjoint s pkey /\
-    LS.rsapss_pkey_pre (v modBits) (v eBits) (as_seq h pkey))
-  (ensures  fun h0 r h1 -> modifies (loc m_def) h0 h1 /\
-    (r, as_seq h1 m_def) == LS.rsapss_verify_bn (v modBits) (v eBits) (as_seq h0 pkey) (as_seq h0 m_def) (as_seq h0 s))
-
-
-inline_for_extraction noextract
-val rsapss_verify_bn: #t:limb_t -> ke:BE.exp t -> modBits:modBits_t t -> rsapss_verify_bn_st t ke modBits
-let rsapss_verify_bn #t ke modBits eBits pkey m_def s =
-  [@inline_let] let bits = size (bits t) in
-  let nLen = blocks modBits bits in
-  let eLen = blocks eBits bits in
-
-  let n  = sub pkey 0ul nLen in
-  let r2 = sub pkey nLen nLen in
-  let e  = sub pkey (nLen +! nLen) eLen in
-
-  let mask = BN.bn_lt_mask nLen s n in
-  let h = ST.get () in
-  SB.bn_lt_mask_lemma (as_seq h s) (as_seq h n);
-
-  let res =
-    if BB.unsafe_bool_of_limb mask then begin
-      Math.Lemmas.pow2_le_compat (v bits * v nLen) (v modBits);
-      SM.bn_precomp_r2_mod_n_lemma (v modBits - 1) (as_seq h n);
-
-      let h0 = ST.get () in
-      BE.mk_bn_mod_exp_precompr2 nLen ke.BE.exp_vt_precomp n r2 s eBits e m_def;
-      let h1 = ST.get () in
-      SD.bn_eval_inj (v nLen) (as_seq h1 m_def)
-        (SE.bn_mod_exp_vartime_precompr2 (v nLen) (as_seq h0 n) (as_seq h0 r2)
-        (as_seq h1 s) (v eBits) (as_seq h0 e));
-
-      if bn_lt_pow2 modBits m_def then true
-      else false end
-    else false in
-  res
-
-
-inline_for_extraction noextract
-let rsapss_verify_bn_to_msg_st (t:limb_t) (a:Hash.hash_alg{S.hash_is_supported a}) (modBits:modBits_t t) =
+let rsapss_verify_msg_st (t:limb_t) (a:Hash.hash_alg{S.hash_is_supported a}) (modBits:modBits_t t) =
+  let emLen = blocks (modBits -! 1ul) 8ul in
     saltLen:size_t
   -> msgLen:size_t
   -> msg:lbuffer uint8 msgLen
-  -> m:lbignum t (blocks modBits (size (bits t))) ->
+  -> em:lbuffer uint8 emLen ->
   Stack bool
   (requires fun h ->
-    live h msg /\ live h m /\ disjoint m msg /\
+    live h msg /\ live h em /\ disjoint em msg /\
 
     LS.rsapss_verify_pre a (v saltLen) (v msgLen) (as_seq h msg))
-  (ensures  fun h0 r h1 -> modifies0 h0 h1 /\
-    r == LS.rsapss_verify_bn_to_msg a (v modBits) (v saltLen) (v msgLen) (as_seq h0 msg) (as_seq h0 m))
+  (ensures  fun h0 r h1 -> modifies0 h0 h1 )
+//    r == LS.rsapss_verify_bn_to_msg a (v modBits) (v saltLen) (v msgLen) (as_seq h0 msg) (as_seq h0 em))
 
 
 inline_for_extraction noextract
-val rsapss_verify_bn_to_msg:
+val rsapss_verify_msg:
     #t:limb_t
   -> a:Hash.hash_alg{S.hash_is_supported a}
   -> modBits:modBits_t t ->
-  rsapss_verify_bn_to_msg_st t a modBits
+  rsapss_verify_msg_st t a modBits
 
-let rsapss_verify_bn_to_msg #t a modBits saltLen msgLen msg m =
-  push_frame ();
-  [@inline_let] let bits : size_pos = bits t in
-  [@inline_let] let numb : size_pos = numbytes t in
-  let nLen = blocks modBits (size bits) in
-
+let rsapss_verify_msg #t a modBits saltLen msgLen msg em =
   let emBits = modBits -! 1ul in
-  let emLen = blocks emBits 8ul in
-  [@inline_let] let mLen = blocks emLen (size numb) in
-  let em = create emLen (u8 0) in
-
-  LS.blocks_bits_lemma t (v emBits);
-  LS.blocks_numb_lemma t (v emBits);
-  assert (SD.blocks (v emBits) bits == v mLen);
-  assert (numb * v mLen <= max_size_t);
-  assert (v mLen <= v nLen);
-
-  let m1 = sub m 0ul mLen in
-  BN.bn_to_bytes_be emLen m1 em;
   let res = RP.pss_verify a saltLen msgLen msg emBits em in
-  pop_frame ();
   res
-
-
-inline_for_extraction noextract
-let rsapss_verify_compute_msg_st (t:limb_t) (ke:BE.exp t) (modBits:modBits_t t) =
-   let len = blocks modBits (size (bits t)) in
-    eBits:size_t{LS.pkey_len_pre t (v modBits) (v eBits)}
-  -> pkey:lbignum t (2ul *! len +! blocks eBits (size (bits t)))
-  -> sgnt:lbuffer uint8 (blocks modBits 8ul)
-  -> m:lbignum t len ->
-  Stack bool
-  (requires fun h -> len == ke.BE.bn.BN.len /\
-    live h sgnt /\ live h pkey /\ live h m /\
-    disjoint m sgnt /\ disjoint m pkey /\
-    as_seq h m == LSeq.create (v len) (uint #t 0) /\
-    LS.rsapss_pkey_pre (v modBits) (v eBits) (as_seq h pkey))
-  (ensures  fun h0 r h1 -> modifies (loc m) h0 h1 /\
-    (r, as_seq h1 m) == LS.rsapss_verify_compute_msg (v modBits) (v eBits) (as_seq h0 pkey) (as_seq h0 sgnt))
-
-
-inline_for_extraction noextract
-val rsapss_verify_compute_msg:
-    #t:limb_t
-  -> ke:BE.exp t
-  -> modBits:modBits_t t ->
-  rsapss_verify_compute_msg_st t ke modBits
-
-let rsapss_verify_compute_msg #t ke modBits eBits pkey sgnt m =
-  push_frame ();
-  [@inline_let] let bits : size_pos = bits t in
-  [@inline_let] let numb : size_pos = numbytes t in
-  let nLen = blocks modBits (size bits) in
-  let k = blocks modBits 8ul in
-
-  let s = create nLen (uint #t 0) in
-  LS.blocks_bits_lemma t (v modBits);
-  LS.blocks_numb_lemma t (v modBits);
-  assert (SD.blocks (v k) numb == v nLen);
-  assert (numb * v nLen <= max_size_t);
-  BN.bn_from_bytes_be k sgnt s;
-
-  let b = rsapss_verify_bn #t ke modBits eBits pkey m s in
-  pop_frame ();
-  b
 
 
 inline_for_extraction noextract
@@ -441,11 +199,11 @@ let rsapss_verify_st1 (t:limb_t) (ke:BE.exp t) (a:Hash.hash_alg{S.hash_is_suppor
     live h msg /\ live h sgnt /\ live h pkey /\
     disjoint msg sgnt /\ disjoint msg pkey /\
 
-    LS.rsapss_pkey_pre (v modBits) (v eBits) (as_seq h pkey) /\
+    LS.rsa_pkey_pre (v modBits) (v eBits) (as_seq h pkey) /\
     LS.rsapss_verify_pre a (v saltLen) (v msgLen) (as_seq h msg))
-  (ensures  fun h0 r h1 -> modifies0 h0 h1 /\
-    r == LS.rsapss_verify_ a (v modBits) (v eBits) (as_seq h0 pkey)
-      (v saltLen) (as_seq h0 sgnt) (v msgLen) (as_seq h0 msg))
+  (ensures  fun h0 r h1 -> modifies0 h0 h1)
+//    r == LS.rsapss_verify_ a (v modBits) (v eBits) (as_seq h0 pkey)
+//      (v saltLen) (as_seq h0 sgnt) (v msgLen) (as_seq h0 msg))
 
 
 inline_for_extraction noextract
@@ -453,16 +211,19 @@ val rsapss_verify_:
     #t:limb_t
   -> ke:BE.exp t
   -> a:Hash.hash_alg{S.hash_is_supported a}
-  -> modBits:modBits_t t ->
+  -> modBits:modBits_t t
+  -> rsa_enc: rsa_enc_st t ke modBits ->
   rsapss_verify_st1 t ke a modBits
 
-let rsapss_verify_ #t ke a modBits eBits pkey saltLen sgnt msgLen msg =
+let rsapss_verify_ #t ke a modBits rsa_enc eBits pkey saltLen sgnt msgLen msg =
   push_frame ();
   [@inline_let] let bits : size_pos = bits t in
   let nLen = blocks modBits (size bits) in
-  let m = create nLen (uint #t 0) in
-  let b = rsapss_verify_compute_msg ke modBits eBits pkey sgnt m in
-  let res = if b then rsapss_verify_bn_to_msg a modBits saltLen msgLen msg m else false in
+  let emBits = modBits -! 1ul in
+  let emLen = blocks emBits 8ul in
+  let em = create emLen (u8 0) in
+  let b = rsa_enc eBits pkey sgnt em in
+  let res = if b then rsapss_verify_msg a modBits saltLen msgLen msg em else false in
   pop_frame ();
   res
 
@@ -482,10 +243,10 @@ let rsapss_verify_st (t:limb_t) (ke:BE.exp t) (a:Hash.hash_alg{S.hash_is_support
     live h msg /\ live h sgnt /\ live h pkey /\
     disjoint msg sgnt /\ disjoint msg pkey /\
 
-    LS.rsapss_pkey_pre (v modBits) (v eBits) (as_seq h pkey))
-  (ensures  fun h0 r h1 -> modifies0 h0 h1 /\
-    r == LS.rsapss_verify a (v modBits) (v eBits) (as_seq h0 pkey)
-      (v saltLen) (v sgntLen) (as_seq h0 sgnt) (v msgLen) (as_seq h0 msg))
+    LS.rsa_pkey_pre (v modBits) (v eBits) (as_seq h pkey))
+  (ensures  fun h0 r h1 -> modifies0 h0 h1)
+//    r == LS.rsapss_verify a (v modBits) (v eBits) (as_seq h0 pkey)
+//      (v saltLen) (v sgntLen) (as_seq h0 sgnt) (v msgLen) (as_seq h0 msg))
 
 
 inline_for_extraction noextract
@@ -493,10 +254,11 @@ val rsapss_verify:
     #t:limb_t
   -> ke:BE.exp t
   -> a:Hash.hash_alg{S.hash_is_supported a}
-  -> modBits:modBits_t t ->
+  -> modBits:modBits_t t
+  -> rsa_enc: rsa_enc_st t ke modBits ->
   rsapss_verify_st t ke a modBits
 
-let rsapss_verify #t ke a modBits eBits pkey saltLen sgntLen sgnt msgLen msg =
+let rsapss_verify #t ke a modBits rsa_enc eBits pkey saltLen sgntLen sgnt msgLen msg =
   let hLen = RM.hash_len a in
   Math.Lemmas.pow2_lt_compat 61 32;
   Math.Lemmas.pow2_lt_compat 125 32;
@@ -509,7 +271,7 @@ let rsapss_verify #t ke a modBits eBits pkey saltLen sgntLen sgnt msgLen msg =
     sgntLen =. blocks modBits 8ul in
 
   if b then
-    rsapss_verify_ ke a modBits eBits pkey saltLen sgnt msgLen msg
+    rsapss_verify_ ke a modBits rsa_enc eBits pkey saltLen sgnt msgLen msg
   else
     false
 
@@ -546,17 +308,17 @@ val rsapss_skey_sign:
   -> ke:BE.exp t
   -> a:Hash.hash_alg{S.hash_is_supported a}
   -> modBits:modBits_t t
-  -> rsapss_load_skey:RK.rsapss_load_skey_st t ke modBits
+  -> rsa_load_skey:RK.rsa_load_skey_st t ke modBits
   -> rsapss_sign:rsapss_sign_st t ke a modBits ->
   rsapss_skey_sign_st t ke a modBits
 
-let rsapss_skey_sign #t ke a modBits rsapss_load_skey rsapss_sign eBits dBits nb eb db saltLen salt msgLen msg sgnt =
+let rsapss_skey_sign #t ke a modBits rsa_load_skey rsapss_sign eBits dBits nb eb db saltLen salt msgLen msg sgnt =
   [@inline_let] let bits = size (bits t) in
   let h0 = ST.get () in
   push_frame ();
   let skey = create (2ul *! blocks modBits bits +! blocks eBits bits +! blocks dBits bits) (uint #t 0) in
-  let b = rsapss_load_skey eBits dBits nb eb db skey in
-  LS.rsapss_load_skey_lemma #t (v modBits) (v eBits) (v dBits) (as_seq h0 nb) (as_seq h0 eb) (as_seq h0 db);
+  let b = rsa_load_skey eBits dBits nb eb db skey in
+  LS.rsa_load_skey_lemma #t (v modBits) (v eBits) (v dBits) (as_seq h0 nb) (as_seq h0 eb) (as_seq h0 db);
 
   let res =
     if b then
@@ -587,9 +349,10 @@ let rsapss_pkey_verify_st (t:limb_t) (ke:BE.exp t) (a:Hash.hash_alg{S.hash_is_su
     live h msg /\ live h sgnt /\ live h nb /\ live h eb /\
     disjoint msg sgnt /\ disjoint nb eb /\ disjoint sgnt nb /\
     disjoint sgnt eb /\ disjoint msg nb /\ disjoint msg eb)
-  (ensures  fun h0 r h1 -> modifies0 h0 h1 /\
-    r == S.rsapss_pkey_verify a (v modBits) (v eBits) (as_seq h0 nb) (as_seq h0 eb)
-      (v saltLen) (v sgntLen) (as_seq h0 sgnt) (v msgLen) (as_seq h0 msg))
+  (ensures  fun h0 r h1 -> modifies0 h0 h1)
+  ///\
+  //  r == S.rsapss_pkey_verify a (v modBits) (v eBits) (as_seq h0 nb) (as_seq h0 eb)
+  //    (v saltLen) (v sgntLen) (as_seq h0 sgnt) (v msgLen) (as_seq h0 msg))
 
 
 inline_for_extraction noextract
@@ -598,17 +361,17 @@ val rsapss_pkey_verify:
   -> ke:BE.exp t
   -> a:Hash.hash_alg{S.hash_is_supported a}
   -> modBits:modBits_t t
-  -> rsapss_load_pkey:RK.rsapss_load_pkey_st t ke modBits
+  -> rsa_load_pkey:RK.rsa_load_pkey_st t ke modBits
   -> rsapss_verify:rsapss_verify_st t ke a modBits ->
   rsapss_pkey_verify_st t ke a modBits
 
-let rsapss_pkey_verify #t ke a modBits rsapss_load_pkey rsapss_verify eBits nb eb saltLen sgntLen sgnt msgLen msg =
+let rsapss_pkey_verify #t ke a modBits rsa_load_pkey rsapss_verify eBits nb eb saltLen sgntLen sgnt msgLen msg =
   push_frame ();
   [@inline_let] let bits = size (bits t) in
   let pkey = create (2ul *! blocks modBits bits +! blocks eBits bits) (uint #t 0) in
   let h0 = ST.get () in
-  let b = rsapss_load_pkey eBits nb eb pkey in
-  LS.rsapss_load_pkey_lemma #t (v modBits) (v eBits) (as_seq h0 nb) (as_seq h0 eb);
+  let b = rsa_load_pkey eBits nb eb pkey in
+  LS.rsa_load_pkey_lemma #t (v modBits) (v eBits) (as_seq h0 nb) (as_seq h0 eb);
 
   let res =
     if b then
@@ -617,6 +380,6 @@ let rsapss_pkey_verify #t ke a modBits rsapss_load_pkey rsapss_verify eBits nb e
       false in
   pop_frame ();
   let h1 = ST.get () in
-  assert (res == LS.rsapss_pkey_verify #t a (v modBits) (v eBits) (as_seq h0 nb) (as_seq h0 eb)
-    (v saltLen) (v sgntLen) (as_seq h0 sgnt) (v msgLen) (as_seq h0 msg));
+//  assert (res == LS.rsapss_pkey_verify #t a (v modBits) (v eBits) (as_seq h0 nb) (as_seq h0 eb)
+//    (v saltLen) (v sgntLen) (as_seq h0 sgnt) (v msgLen) (as_seq h0 msg));
   res
