code/rsapss/Hacl.Impl.RSA.fst
@@ -1,0 +1,270 @@
+module Hacl.Impl.RSA
+
+open FStar.HyperStack
+open FStar.HyperStack.ST
+open FStar.Mul
+
+open Lib.IntTypes
+open Lib.Buffer
+
+open Hacl.Bignum.Definitions
+
+module ST = FStar.HyperStack.ST
+
+module Hash = Spec.Agile.Hash
+module SB = Hacl.Spec.Bignum
+module BB = Hacl.Spec.Bignum.Base
+module SD = Hacl.Spec.Bignum.Definitions
+module SM = Hacl.Spec.Bignum.Montgomery
+module SE = Hacl.Spec.Bignum.Exponentiation
+
+module BN = Hacl.Bignum
+module BE = Hacl.Bignum.Exponentiation
+module BM = Hacl.Bignum.Montgomery
+
+module S = Spec.RSAPSS
+module LS = Hacl.Spec.RSAPSS
+module LSeq = Lib.Sequence
+
+module RK = Hacl.Impl.RSA.Keys
+
+#reset-options "--z3rlimit 150 --fuel 0 --ifuel 0"
+
+inline_for_extraction noextract
+let modBits_t (t:limb_t) = modBits:size_t{1 < v modBits /\ 2 * bits t * SD.blocks (v modBits) (bits t) <= max_size_t}
+
+
+inline_for_extraction noextract
+let rsa_dec_bn_st (t:limb_t) (ke:BE.exp t) (modBits:modBits_t t) =
+  let len = blocks modBits (size (bits t)) in
+    eBits:size_t
+  -> dBits:size_t{LS.skey_len_pre t (v modBits) (v eBits) (v dBits)}
+  -> skey:lbignum t (2ul *! len +! blocks eBits (size (bits t)) +! blocks dBits (size (bits t)))
+  -> m:lbignum t len
+  -> m':lbignum t len
+  -> s:lbignum t len ->
+  Stack bool
+  (requires fun h -> len == ke.BE.bn.BN.len /\
+    live h skey /\ live h m /\ live h s /\ live h m' /\
+    disjoint s m /\ disjoint s skey /\ disjoint m skey /\
+    disjoint m m' /\ disjoint m' s /\ disjoint m' skey /\
+    LS.rsa_skey_pre (v modBits) (v eBits) (v dBits) (as_seq h skey) /\
+    bn_v h m < bn_v h (gsub skey 0ul len))
+  (ensures  fun h0 r h1 -> modifies (loc s |+| loc m') h0 h1 /\
+    (r, as_seq h1 s) == LS.rsapss_sign_bn (v modBits) (v eBits) (v dBits) (as_seq h0 skey) (as_seq h0 m))
+
+
+inline_for_extraction noextract
+val rsa_dec_bn: #t:limb_t -> ke:BE.exp t -> modBits:modBits_t t -> rsa_dec_bn_st t ke modBits
+let rsa_dec_bn #t ke modBits eBits dBits skey m m' s =
+  [@inline_let] let bits : size_pos = bits t in
+  let nLen = blocks modBits (size bits) in
+  let eLen = blocks eBits (size bits) in
+  let dLen = blocks dBits (size bits) in
+
+  let n  = sub skey 0ul nLen in
+  let r2 = sub skey nLen nLen in
+  let e  = sub skey (nLen +! nLen) eLen in
+  let d  = sub skey (nLen +! nLen +! eLen) dLen in
+
+  Math.Lemmas.pow2_le_compat (bits * v nLen) (v modBits);
+  let h0 = ST.get () in
+  SM.bn_precomp_r2_mod_n_lemma (v modBits - 1) (as_seq h0 n);
+  BE.mk_bn_mod_exp_precompr2 nLen ke.BE.exp_ct_precomp n r2 m dBits d s;
+  BE.mk_bn_mod_exp_precompr2 nLen ke.BE.exp_vt_precomp n r2 s eBits e m';
+  let h1 = ST.get () in
+  SD.bn_eval_inj (v nLen) (as_seq h1 s)
+    (SE.bn_mod_exp_consttime_precompr2 (v nLen) (as_seq h0 n) (as_seq h0 r2)
+    (as_seq h0 m) (v dBits) (as_seq h0 d));
+  SD.bn_eval_inj (v nLen) (as_seq h1 m')
+    (SE.bn_mod_exp_vartime_precompr2 (v nLen) (as_seq h0 n) (as_seq h0 r2)
+    (as_seq h1 s) (v eBits) (as_seq h0 e));
+  let eq_m = BN.bn_eq_mask nLen m m' in
+  mapT nLen s (logand eq_m) s;
+  BB.unsafe_bool_of_limb eq_m
+
+
+inline_for_extraction noextract
+let rsa_dec_st (t:limb_t) (ke:BE.exp t) (modBits:modBits_t t) =
+  let len = blocks modBits (size (bits t)) in
+  let emLen = blocks (modBits -! 1ul) 8ul in
+    eBits:size_t
+  -> dBits:size_t{LS.skey_len_pre t (v modBits) (v eBits) (v dBits)}
+  -> skey:lbignum t (2ul *! len +! blocks eBits (size (bits t)) +! blocks dBits (size (bits t)))
+  -> em:lbuffer uint8 emLen
+  -> sgnt:lbuffer uint8 (blocks modBits 8ul) ->
+  Stack bool
+  (requires fun h -> len == ke.BE.bn.BN.len /\
+    live h sgnt /\ live h skey /\ live h em /\
+    disjoint sgnt skey /\ disjoint em sgnt /\ disjoint em skey /\
+    LS.rsa_skey_pre (v modBits) (v eBits) (v dBits) (as_seq h skey) /\
+    (let emBits = v modBits - 1 in
+      if emBits % 8 > 0 then v (Seq.index (as_seq h em) 0) < pow2 (emBits % 8) else v (Seq.index (as_seq h em) 0) < pow2 8))
+  (ensures  fun h0 eq_m h1 -> modifies (loc sgnt) h0 h1 /\
+    (eq_m, as_seq h1 sgnt) == 
+    LS.rsapss_sign_compute_sgnt #t (v modBits) (v eBits) (v dBits) (as_seq h0 skey) (as_seq h0 em))
+
+
+inline_for_extraction noextract
+val rsa_dec:
+    #t:limb_t
+  -> ke:BE.exp t
+  -> modBits:modBits_t t ->
+  rsa_dec_st t ke modBits
+
+#push-options "--z3rlimit 200"
+let rsa_dec #t ke modBits eBits dBits skey em sgnt =
+  push_frame ();
+  [@inline_let] let bits : size_pos = bits t in
+  [@inline_let] let numb : size_pos = numbytes t in
+  let nLen = blocks modBits (size bits) in
+  let emBits = modBits -! 1ul in
+  let emLen = blocks emBits 8ul in
+  [@inline_let] let mLen = blocks emLen (size numb) in
+  let k = blocks modBits 8ul in
+  
+  LS.blocks_bits_lemma t (v emBits);
+  LS.blocks_numb_lemma t (v emBits);
+  assert (SD.blocks (v emBits) bits = v mLen);
+  assert (numb * v mLen <= max_size_t);
+  assert (v mLen <= v nLen);
+
+  let m = create nLen (uint #t 0) in
+  let s = create nLen (uint #t 0) in
+  let m' = create nLen (uint #t 0) in
+  let h' = ST.get () in
+  update_sub_f h' m 0ul mLen
+    (fun h -> SB.bn_from_bytes_be (v emLen) (as_seq h' em))
+    (fun _ -> BN.bn_from_bytes_be emLen em (sub m 0ul mLen));
+  let h = ST.get() in
+  assume (bn_v h m < bn_v h (gsub skey 0ul nLen));
+  let eq_b = rsa_dec_bn ke modBits eBits dBits skey m m' s in
+  LS.blocks_bits_lemma t (v modBits);
+  LS.blocks_numb_lemma t (v modBits);
+  assert (SD.blocks (v k) numb == v nLen);
+  assert (numb * v nLen <= max_size_t);
+  BN.bn_to_bytes_be k s sgnt;
+  pop_frame ();
+  eq_b
+#pop-options
+
+
+inline_for_extraction noextract
+val bn_lt_pow2:
+    #t:limb_t
+  -> modBits:size_t{1 < v modBits}
+  -> m:lbignum t (blocks modBits (size (bits t))) ->
+  Stack bool
+  (requires fun h -> live h m)
+  (ensures  fun h0 r h1 -> h0 == h1 /\
+    r == LS.bn_lt_pow2 (v modBits) (as_seq h0 m))
+
+let bn_lt_pow2 #t modBits m =
+  if not ((modBits -! 1ul) %. 8ul =. 0ul) then true
+  else begin
+    let get_bit = BN.bn_get_ith_bit (blocks modBits (size (bits t))) m (modBits -! 1ul) in
+    BB.unsafe_bool_of_limb0 get_bit end
+
+
+inline_for_extraction noextract
+let rsa_enc_bn_st (t:limb_t) (ke:BE.exp t) (modBits:modBits_t t) =
+  let len = blocks modBits (size (bits t)) in
+    eBits:size_t{LS.pkey_len_pre t (v modBits) (v eBits)}
+  -> pkey:lbignum t (2ul *! len +! blocks eBits (size (bits t)))
+  -> s:lbignum t len
+  -> m_def:lbignum t len ->
+  Stack bool
+  (requires fun h -> len == ke.BE.bn.BN.len /\
+    live h pkey /\ live h m_def /\ live h s /\
+    disjoint m_def pkey /\ disjoint m_def s /\ disjoint s pkey /\
+    LS.rsa_pkey_pre (v modBits) (v eBits) (as_seq h pkey))
+  (ensures  fun h0 r h1 -> modifies (loc m_def) h0 h1 /\
+    (r, as_seq h1 m_def) == LS.rsapss_verify_bn (v modBits) (v eBits) (as_seq h0 pkey) (as_seq h0 m_def) (as_seq h0 s))
+
+
+inline_for_extraction noextract
+val rsa_enc_bn: #t:limb_t -> ke:BE.exp t -> modBits:modBits_t t -> rsa_enc_bn_st t ke modBits
+let rsa_enc_bn #t ke modBits eBits pkey s m_def =
+  [@inline_let] let bits = size (bits t) in
+  let nLen = blocks modBits bits in
+  let eLen = blocks eBits bits in
+
+  let n  = sub pkey 0ul nLen in
+  let r2 = sub pkey nLen nLen in
+  let e  = sub pkey (nLen +! nLen) eLen in
+
+  let mask = BN.bn_lt_mask nLen s n in
+  let h = ST.get () in
+  SB.bn_lt_mask_lemma (as_seq h s) (as_seq h n);
+
+  let res =
+    if BB.unsafe_bool_of_limb mask then begin
+      Math.Lemmas.pow2_le_compat (v bits * v nLen) (v modBits);
+      SM.bn_precomp_r2_mod_n_lemma (v modBits - 1) (as_seq h n);
+
+      let h0 = ST.get () in
+      BE.mk_bn_mod_exp_precompr2 nLen ke.BE.exp_vt_precomp n r2 s eBits e m_def;
+      let h1 = ST.get () in
+      SD.bn_eval_inj (v nLen) (as_seq h1 m_def)
+        (SE.bn_mod_exp_vartime_precompr2 (v nLen) (as_seq h0 n) (as_seq h0 r2)
+        (as_seq h1 s) (v eBits) (as_seq h0 e));
+
+      if bn_lt_pow2 modBits m_def then true
+      else false end
+    else false in
+  res
+
+
+inline_for_extraction noextract
+let rsa_enc_st (t:limb_t) (ke:BE.exp t) (modBits:modBits_t t) =
+   let len = blocks modBits (size (bits t)) in
+   let emLen = blocks (modBits -! 1ul) 8ul in
+    eBits:size_t{LS.pkey_len_pre t (v modBits) (v eBits)}
+  -> pkey:lbignum t (2ul *! len +! blocks eBits (size (bits t)))
+  -> sgnt:lbuffer uint8 (blocks modBits 8ul)
+  -> em:lbuffer uint8 emLen ->
+  Stack bool
+  (requires fun h -> len == ke.BE.bn.BN.len /\
+    live h sgnt /\ live h pkey /\ live h em /\
+    disjoint em sgnt /\ disjoint em pkey /\
+    as_seq h em == LSeq.create (v emLen) (u8 0) /\
+    LS.rsa_pkey_pre (v modBits) (v eBits) (as_seq h pkey))
+  (ensures  fun h0 r h1 -> modifies (loc em) h0 h1)
+//    (r, as_seq h1 em) == LS.rsapss_verify_compute_msg (v modBits) (v eBits) (as_seq h0 pkey) (as_seq h0 sgnt))
+
+
+inline_for_extraction noextract
+val rsa_enc:
+    #t:limb_t
+  -> ke:BE.exp t
+  -> modBits:modBits_t t ->
+  rsa_enc_st t ke modBits
+
+let rsa_enc #t ke modBits eBits pkey sgnt em =
+  push_frame ();
+  [@inline_let] let bits : size_pos = bits t in
+  [@inline_let] let numb : size_pos = numbytes t in
+  let nLen = blocks modBits (size bits) in
+  let k = blocks modBits 8ul in
+
+
+  let emBits = modBits -! 1ul in
+  let emLen = blocks emBits 8ul in
+  
+  let s = create nLen (uint #t 0) in
+  let m = create (blocks (modBits) (size bits)) (uint #t 0) in
+  
+  LS.blocks_bits_lemma t (v modBits);
+  LS.blocks_numb_lemma t (v modBits);
+  assert (SD.blocks (v k) numb == v nLen);
+  assert (numb * v nLen <= max_size_t);
+  BN.bn_from_bytes_be k sgnt s;
+
+  let b = rsa_enc_bn #t ke modBits eBits pkey s m in
+
+  [@inline_let] let mLen = blocks emLen (size numb) in
+  let m1 = sub m 0ul mLen in
+  BN.bn_to_bytes_be emLen m1 em;
+  pop_frame ();
+  b
+
